pulse/share/steel/examples/pulse/lib/Pulse.Lib.HashTable.fst
@@ -5,8 +5,7 @@ module R = Pulse.Lib.Reference
 module US = FStar.SizeT
 module U8 = FStar.UInt8
 module U64 = FStar.UInt64
-module PHT = LinearScanHashTable
-open LinearScanHashTable
+module PHT = LinearProbeHashTable
 open Pulse.Class.BoundedIntegers
 
 #push-options "--using_facts_from '* -FStar.Tactics -FStar.Reflection'"
@@ -43,8 +42,14 @@ fn _alloc (#s:pht_sig_us) (l:pos_us)
 ```
 let alloc #s l = _alloc #s l
 
+let perform (#a:Type0) (#b:Type0) (f:  (a -> stt b emp (fun _ -> emp))) (x:a) 
+  : stt b emp (fun _ -> emp)
+  = f x
+
 ```pulse
-fn _dealloc (#s:pht_sig_us) (ht:ht_t s) (l:pos_us) (destroy_val:destroy_val_fn_t s.valt)
+fn _dealloc (#s:pht_sig_us) (ht:ht_t s) (l:pos_us) 
+  (destroy_val:destroy_fn_t s.valt)
+  (destroy_key:destroy_fn_t s.keyt)
   requires exists pht. models s ht pht
   ensures emp
 {
@@ -68,8 +73,8 @@ fn _dealloc (#s:pht_sig_us) (ht:ht_t s) (l:pos_us) (destroy_val:destroy_val_fn_t
     let c = (ht.contents).(voff);
     match c {
       Used k v -> {
-        // TODO: destroy key as well
-        destroy_val v;
+        perform destroy_val v;
+        perform destroy_key k;
       }
       _ -> {
         off := voff + 1sz;
